theories/L/Complexity/Cook/GenNP_PR_Tape.v
@@ -1,0 +1,670 @@
+(* -*- company-coq-local-symbols: (("|_|" .?␣)); -*- *)
+From PslBase Require Import FiniteTypes. 
+From Undecidability.TM Require Import TM.
+Require Import Lia. 
+From Undecidability.L.Complexity.Cook Require Import GenNP TCSR Prelim GenNP_PR_Basics.
+
+Module tape (sig : TMSig).
+  Module basics' := basics sig.
+  Export basics'.
+
+  (*For easier automation, we define the rewrite rules using inductive predicates *)
+  Section fixRulePred.
+    (*We define the equivalent of rewritesHeadList for predicate-based rules  *)
+
+    Context {X : Type}.
+    Context (p : X -> X -> X -> X -> X -> X -> Prop). 
+
+    Inductive rewritesHeadInd: list X -> list X -> Prop :=
+      | rewHead_indC (x1 x2 x3 x4 x5 x6 : X) s1 s2 : p x1 x2 x3 x4 x5 x6 -> rewritesHeadInd (x1 :: x2 :: x3 :: s1) (x4 :: x5 :: x6 :: s2). 
+
+    Hint Constructors rewritesHeadInd. 
+
+    (*a few facts which will be useful *)
+    Lemma rewritesHeadInd_tail_invariant (γ1 γ2 γ3 γ4 γ5 γ6 : X) s1 s2 s1' s2' :
+      rewritesHeadInd (γ1 :: γ2 :: γ3 :: s1) (γ4 :: γ5 :: γ6 :: s2) <-> rewritesHeadInd (γ1 :: γ2 :: γ3 :: s1') (γ4 :: γ5 :: γ6 :: s2').
+    Proof. split; intros; inv H; eauto. Qed. 
+
+    Corollary rewritesHeadInd_rem_tail (γ1 γ2 γ3 γ4 γ5 γ6 : X) h1 h2 :
+      rewritesHeadInd [γ1; γ2; γ3] [γ4; γ5; γ6] <-> rewritesHeadInd (γ1 :: γ2 :: γ3 :: h1) (γ4 :: γ5 :: γ6 :: h2).
+    Proof. now apply rewritesHeadInd_tail_invariant. Qed. 
+
+    Lemma rewritesHeadInd_append_invariant (γ1 γ2 γ3 γ4 γ5 γ6 : X) s1 s2 s1' s2' :
+      rewritesHeadInd (γ1 :: γ2 :: γ3 :: s1) (γ4 :: γ5 :: γ6 :: s2) <-> rewritesHeadInd (γ1 :: γ2 :: γ3 :: s1 ++ s1') (γ4 :: γ5 :: γ6 :: s2 ++ s2').
+    Proof. now apply rewritesHeadInd_tail_invariant. Qed.
+
+    Lemma rewritesAt_rewritesHeadInd_add_at_end i a b h1 h2 :
+      rewritesAt rewritesHeadInd i a b -> rewritesAt rewritesHeadInd i (a ++ h1) (b ++ h2).
+    Proof. 
+      intros. unfold rewritesAt in *. inv H; symmetry in H0; symmetry in H1; repeat erewrite skipn_app2; eauto; try congruence; cbn; eauto. 
+    Qed.
+
+    Lemma rewritesAt_rewritesHeadInd_rem_at_end i a b h1 h2 :
+      rewritesAt rewritesHeadInd i (a ++ h1) (b ++ h2) -> i < |a| - 2 -> i < |b| - 2 -> rewritesAt rewritesHeadInd i a b.
+    Proof. 
+      intros. unfold rewritesAt in *.
+      assert (i <= |a|) by lia. destruct (skipn_app3 h1 H2) as (a' & H3 & H4). rewrite H3 in H. 
+      assert (i <= |b|) by lia. destruct (skipn_app3 h2 H5) as (b' & H6 & H7). rewrite H6 in H. 
+      clear H2 H5.
+      rewrite <- firstn_skipn with (l := a) (n := i) in H4 at 1. apply app_inv_head in H4 as <-. 
+      rewrite <- firstn_skipn with (l := b) (n := i) in H7 at 1. apply app_inv_head in H7 as <-. 
+      specialize (skipn_length i a) as H7. specialize (skipn_length i b) as H8. 
+      remember (skipn i a) as l. do 3 (destruct l as [ | ? l] ; [cbn in H7; lia | ]). 
+      remember (skipn i b) as l'. do 3 (destruct l' as [ | ? l']; [cbn in H8; lia | ]). 
+      cbn in H. rewrite rewritesHeadInd_tail_invariant in H. apply H. 
+    Qed. 
+  End fixRulePred. 
+
+  Hint Constructors rewritesHeadInd.
+
+  (*unfold the three symbols at the head of premise and conclusion of a rewrite rule *)
+  Ltac rewritesHeadInd_inv := 
+    repeat match goal with
+    | [H : rewritesHeadInd _ ?a _ |- _] => is_var a; destruct a; try (inv H; fail)
+    | [H : rewritesHeadInd _ (_ :: ?a) _ |- _] => is_var a; destruct a; try (inv H; fail)
+    | [H : rewritesHeadInd _ (_ :: _ :: ?a) _ |- _] => is_var a; destruct a; try (inv H; fail)
+    | [H : rewritesHeadInd _ _ ?a |- _ ] => is_var a; destruct a; try (inv H; fail)
+    | [H : rewritesHeadInd _ _ (_ :: ?a) |-_ ] => is_var a; destruct a; try (inv H; fail)
+    | [H : rewritesHeadInd _ _ (_ :: _ :: ?a) |- _] => is_var a; destruct a; try (inv H; fail)
+    end.
+
+(* Section tape.  *)
+(*   Context {inst : GenNPInstance}.  *)
+
+(*   Definition inst' := Build_GenNPInstance (@trans inst) (@halt inst) (@start inst) (@t inst) (@k inst). *)
+
+(*   Canonical Structure inst'. *)
+
+(*   (* Notation states := (states inst).  *) *)
+(*   (* Notation Sigma := (Sigma inst).  *) *)
+(*   (* Notation trans := (@trans inst). *) *)
+
+(*   (* Notation t := (t inst). *) *)
+(*   (* Notation k := (k inst).  *) *)
+
+(*   Notation sconfig := (sconfig states Sigma).  *)
+(*   Notation sstep := (sstep trans). *)
+
+(*   Notation polarity := move.  *)
+(*   Notation positive := R.  *)
+(*   Notation negative := L.  *)
+(*   Notation neutral := N.  *)
+
+(*   Notation "'↓' σ" := ((negative, σ)) (at level 30).  *)
+(*   Notation "'↑' σ" := ((positive, σ)) (at level 30). *)
+(*   Notation "'∘' σ" := ((neutral, σ)) (at level 30).  *)
+
+(*   Notation "$" := (inl delimC).  *)
+(*   Notation "'|_|'" := (None).  *)
+
+
+(*   Notation "p ! a" := (withPolarity p a) (at level 5).  *)
+(*   Notation "p !! a" := (withPolaritySigma p a) (at level 5).  *)
+
+
+  (** *inductive rule predicates for tape rewrites *)
+
+  (*the rules for shifting the tape to the right *)
+  Inductive shiftRightRules : Gamma -> Gamma -> Gamma -> Gamma -> Gamma -> Gamma -> Prop :=
+    | shiftRightSSSS σ1 σ2 σ3 σ4 p : shiftRightRules (inr (inr (p, Some σ1))) (inr (inr (p, Some σ2))) (inr (inr (p, Some σ3))) (inr (inr (positive, Some σ4))) (inr (inr (positive, Some σ1))) (inr (inr (positive, Some σ2))) 
+    | shiftRightBBBS p σ1 : shiftRightRules (inr (inr (p, |_|))) (inr (inr (p, |_|))) (inr (inr (p, |_|))) (inr (inr (positive, Some σ1))) (inr (inr (positive, |_|))) (inr (inr (positive, |_|)))
+    | shiftRightBBBB p : shiftRightRules (inr (inr (p, |_|))) (inr (inr (p, |_|))) (inr (inr (p, |_|))) (inr (inr (positive, |_|))) (inr (inr (positive, |_|))) (inr (inr (positive, |_|)))
+    | shiftRightSBB σ1 σ2 p : shiftRightRules (inr (inr (p, Some σ1))) (inr (inr (p, |_|))) (inr (inr (p, |_|))) (inr (inr (positive, Some σ2))) (inr (inr (positive, Some σ1))) (inr (inr (positive, |_|)))
+    | shiftRightSSB σ1 σ2 σ3 p : shiftRightRules (inr (inr (p, Some σ1))) (inr (inr (p, Some σ2))) (inr (inr (p, |_|))) (inr (inr (positive, Some σ3))) (inr (inr (positive, Some σ1))) (inr (inr (positive, Some σ2))) 
+    | shiftRightBBS σ1 p : shiftRightRules (inr (inr (p, |_|))) (inr (inr (p, |_|))) (inr (inr (p, Some σ1))) (inr (inr (positive, |_|))) (inr (inr (positive, |_|))) (inr (inr (positive, |_|)))
+    | shiftRightBSS σ1 σ2 p : shiftRightRules (inr (inr (p, |_|))) (inr (inr (p, Some σ1))) (inr (inr (p, Some σ2))) (inr (inr (positive, |_|))) (inr (inr (positive, |_|))) (inr (inr (positive, Some σ1)))
+    | shiftRightSSSB σ1 σ2 σ3 p : shiftRightRules (inr (inr (p, Some σ1))) (inr (inr (p, Some σ2))) (inr (inr (p, Some σ3))) (inr (inr (positive, |_|))) (inr (inr (positive, Some σ1))) (inr (inr (positive, Some σ2))).
+
+  Hint Constructors shiftRightRules. 
+
+  (*identity rules *)
+  Inductive identityRules : Gamma -> Gamma -> Gamma -> Gamma -> Gamma -> Gamma -> Prop :=
+    | identityC (m1 m2 m3 : stateSigma) p : identityRules (inr (inr (p, m1))) (inr (inr (p, m2))) (inr (inr (p, m3))) (inr (inr (neutral, m1))) (inr (inr (neutral, m2))) (inr (inr (neutral, m3)))
+  | identityDBB p p' : identityRules (inr #) (inr (inr (p, |_|))) (inr (inr (p, |_|))) (inr #) (inr (inr (p', |_|))) (inr (inr (p', |_|)))
+  | identityBBD p p' : identityRules (inr (inr (p, |_|))) (inr (inr (p, |_|))) (inr #) (inr (inr (p', |_|))) (inr (inr (p', |_|))) (inr #). 
+
+  Hint Constructors identityRules.
+
+  (*the rules for shifting the tape left are derived from the ones for right shifts using reversion and polarity flips *)
+  Inductive tapeRules : Gamma -> Gamma -> Gamma -> Gamma -> Gamma -> Gamma -> Prop :=
+  | shiftLeftTapeC γ1 γ2 γ3 γ4 γ5 γ6: shiftRightRules (~γ3) (~γ2) (~γ1) (~γ6) (~γ5) (~γ4) -> tapeRules γ1 γ2 γ3 γ4 γ5 γ6
+  | shiftRightTapeC γ1 γ2 γ3 γ4 γ5 γ6: shiftRightRules γ1 γ2 γ3 γ4 γ5 γ6 -> tapeRules γ1 γ2 γ3 γ4 γ5 γ6
+  | identityTapeC γ1 γ2 γ3 γ4 γ5 γ6: identityRules γ1 γ2 γ3 γ4 γ5 γ6 -> tapeRules γ1 γ2 γ3 γ4 γ5 γ6. 
+
+  Hint Constructors tapeRules. 
+
+  Notation rewHeadTape := (rewritesHeadInd tapeRules).
+
+  (*since the rules for shifting left are derived from the rules for shifting right using polarityFlipGamma, the polarity flip functions need to be reduced in order to be able to apply the constructors *)
+  Hint Extern 4 (tapeRules _ _ _ _ _ _) => apply shiftLeftTapeC;
+  cbn [polarityFlipGamma polarityFlipTapeSigma polarityFlipSigma polarityFlip].
+
+
+  Ltac rewHeadTape_inv1 :=
+    repeat match goal with
+    | [H : rewHeadTape _ _ |- _] => inv H
+    | [H : tapeRules _ _ _ _ _ _ |- _] => inv H
+    end.
+
+  (*identity rules are invariant under polarity flip + reversion *)
+  Lemma identityWindow_revp (γ1 γ2 γ3 γ4 γ5 γ6 : Gamma) : identityRules γ1 γ2 γ3 γ4 γ5 γ6 <-> identityRules (~γ3) (~γ2) (~γ1) (~γ6) (~γ5) (~γ4).
+  Proof.
+    split; intros; inv H; cbn.
+    all: repeat match goal with
+           | [H : delim |- _] => destruct H
+           | [H : inr _ = (~ _) |- _] => symmetry in H
+           | [H : inr _ = inr _ |- _] => inv H
+           | [H : inl _ = inl _ |- _] => inv H
+           | [H : (~ ?a) = inr (#) |- _ ] => is_var a; destruct a; cbn in H; [congruence | ]
+           | [H : % ?a = # |- _] => is_var a; destruct a; cbn in H; try congruence
+           | [H : (~ _)= inr(inr ((_, _))) |- _] => apply polarityFlipGammaInv1 in H as ->
+                end; try congruence.
+    all: eauto. 
+  Qed. 
+
+  (*in fact, all tape rules are invariant under polarity flip + reversion: for the shift rules, this directly follows from the definition *)
+  Lemma tapeRules_revp' γ1 γ2 γ3 γ4 γ5 γ6 : tapeRules γ1 γ2 γ3 γ4 γ5 γ6 -> tapeRules (~γ3) (~γ2) (~γ1) (~γ6) (~γ5) (~γ4). 
+  Proof. 
+    intros. rewHeadTape_inv1. 
+    - eauto. 
+    - constructor. now rewrite !polarityFlipGamma_involution.
+    - apply identityWindow_revp in H0. eauto.  
+  Qed. 
+
+  Lemma tapeRules_revp γ1 γ2 γ3 γ4 γ5 γ6 : tapeRules γ1 γ2 γ3 γ4 γ5 γ6 <-> tapeRules (~γ3) (~γ2) (~γ1) (~γ6) (~γ5) (~γ4).
+  Proof. 
+    split.
+    apply tapeRules_revp'. intros H%tapeRules_revp'.
+    specialize polarityFlipGamma_involution as H1. unfold involution in H1.
+    now repeat rewrite H1 in H.
+  Qed.
+
+  (*inversion of the tape rules *)
+  Ltac rewHeadTape_inv2 :=
+    repeat match goal with
+      | [H : rewHeadTape _ _ |- _ ] => inv H
+      | [H : tapeRules _ _ _ _ _ _ |- _] => inv H
+      | [H : shiftRightRules _ _ _ _ _ _ |- _ ] => inv H
+      | [H : identityRules _ _ _ _ _ _ |- _] => inv H
+      | [d : delim |- _] => destruct d
+      | [H : (~?e) = inr (inr (_, _)) |- _] => apply polarityFlipGammaInv1 in H; try rewrite H in *; clear H
+      | [H : inr (inr (_, _)) = (~?e) |- _] => symmetry in H; apply polarityFlipGammaInv1 in H; try rewrite H in *; clear H
+      | [H : inr _ = inr _ |- _] => inv H
+      | [H : inl _ = inl _ |- _] => inv H
+    end; try congruence. 
+ 
+  (*the following lemmas allow us to prove results only for the right tape half and derive the corresponding results for the left tape half as corollaries *)
+  (*Lemma 15 *)
+  Lemma tape_rewrite_symm1 h h' :
+    valid rewHeadTape h h' -> valid rewHeadTape (polarityRev h) (polarityRev h').
+  Proof.
+    intros.  
+    induction H; intros. 
+    - cbn; constructor. 
+    - apply valid_length_inv in H.
+      destruct a, b; try destruct a; try destruct b; cbn in *; try lia. all: repeat constructor. 
+    - rewritesHeadInd_inv; cbn. 
+      rewrite valid_iff. unfold validExplicit. repeat rewrite app_length.
+      repeat rewrite rev_length, map_length. cbn [length]. split.
+      1: apply valid_length_inv in H; now cbn [length] in H. 
+      replace ((|a|) + 1 + 1 + 1 - 2) with (S (|a|)) by lia. intros. destruct (nat_eq_dec i (|a|)) as [-> | F]. 
+      * (*rewrite at the new position, cannot apply IH *)
+        unfold rewritesAt. 
+        apply rewritesHeadInd_rem_tail in H0.
+        inv H0. apply tapeRules_revp' in H3. 
+        cbn [rev map].
+        repeat rewrite <- app_assoc.
+        rewrite skipn_app with (xs := rev (map polarityFlipGamma a)).
+        rewrite skipn_app with (xs := rev (map polarityFlipGamma b)).
+        2, 3: rewrite rev_length, map_length. 3: reflexivity. 
+        2: { apply valid_length_inv in H; cbn [length] in H. lia. }
+        cbn. constructor. apply H3. 
+      * (*this follows by IH *)
+        cbn [polarityRev map rev] in IHvalid. 
+        apply valid_iff in IHvalid as (IH1 & IH2). 
+        assert (0 <= i < |a|) by lia. 
+        repeat rewrite app_length in IH2. rewrite rev_length, map_length in IH2. cbn [length] in IH2.
+        replace ((|a|) + 1 + 1 - 2) with (|a|) in IH2 by lia. 
+        specialize (IH2 i H2).
+        apply rewritesAt_rewritesHeadInd_add_at_end. apply IH2. 
+  Qed. 
+
+  Lemma tape_rewrite_symm2 h h' : valid rewHeadTape (polarityRev h) (polarityRev h') -> valid rewHeadTape h h'.
+  Proof.
+    intros. specialize (tape_rewrite_symm1 H) as H1. now repeat rewrite polarityRev_involution in H1.
+  Qed. 
+
+  Lemma tape_rewrite_symm3 h h' : valid rewHeadTape h h' -> valid rewHeadTape (map polarityFlipGamma h) h'. 
+  Proof. 
+    intros. unfold reprTape in H. induction H; intros. 
+    - cbn; constructor. 
+    - cbn; constructor. 2: now rewrite map_length. apply IHvalid.  
+    - cbn. rewritesHeadInd_inv. constructor 3.
+      + apply IHvalid. 
+      + cbn. apply rewritesHeadInd_rem_tail.
+        rewHeadTape_inv2; cbn; eauto 100.  
+  Qed.
+
+  (*Lemma 16 *)
+  Lemma E_rewrite_blank p p' n: valid rewHeadTape (E p (S (S n))) (E p' (S (S n))). 
+  Proof. 
+    intros. induction n. 
+    + apply valid_base. eauto. 
+    + constructor 3. 
+      - cbn [E] in IHn. now apply IHn. 
+      - destruct p'; eauto. 
+  Qed. 
+
+  (*blank rewriting is uniquely determined if the head of the target is known *)
+  Lemma E_rewrite_blank_unique' p p' n : n >= 1 -> forall s, valid rewHeadTape (E p' (S n)) (inr (inr (p, |_|)) :: s) -> s = E p n. 
+  Proof. 
+    intros H. induction n; intros; [lia | ]. 
+    destruct n; cbn [E] in *. 
+    + inv_valid. rewHeadTape_inv2. 
+      apply valid_length_inv in H4. inv H4. now (destruct s2; cbn in H1).
+    + inv_valid. rewHeadTape_inv2.
+      1-2: cbn in *; destruct p; cbn in H5; try congruence; clear H5.
+      all: apply IHn in H4; [congruence | lia]. 
+  Qed. 
+
+  Corollary E_rewrite_blank_unique p p' n : forall s, valid rewHeadTape (E p (S (S n))) (inr (inr (p', |_|)) :: s) -> s = E p' (S n).
+  Proof. intros; now eapply E_rewrite_blank_unique'. Qed.
+
+  (*the same results for the left tape half *)
+  Lemma E_rewrite_blank_rev p p' w : valid rewHeadTape (rev (E p (S (S w)))) (rev (E p' (S (S w)))).  
+  Proof. 
+    rewrite <- polarityFlip_involution with (x := p). rewrite <- polarityFlip_involution with (x := p'). 
+    rewrite <- !E_polarityFlip. apply tape_rewrite_symm1. rewrite !E_polarityFlip. apply E_rewrite_blank.
+  Qed. 
+
+  Lemma E_rewrite_blank_rev_unique p p' w s : valid rewHeadTape (rev (E p (S (S w)))) (rev (inr (inr (p', |_|)) :: s)) -> s = (E p' (S (w))). 
+  Proof. 
+    intros.
+    assert (valid rewHeadTape (polarityRev (E (polarityFlip p) (S (S w)))) (polarityRev (map polarityFlipGamma (inr (inr (p', |_|)) :: s)))). 
+    {
+      unfold polarityRev. rewrite E_polarityFlip. rewrite map_involution. 2: involution_simpl. rewrite polarityFlip_involution. apply H.
+    }
+    apply tape_rewrite_symm2 in H0.
+    cbn in H0. apply E_rewrite_blank_unique in H0.
+    apply involution_invert_eqn2 with (a := s) (f:= (map polarityFlipGamma))  (b := E (polarityFlip p') (S w)) in H0.
+    2: involution_simpl. now rewrite H0, E_polarityFlip, polarityFlip_involution. 
+  Qed. 
+
+  (*Lemma 17 *)
+  (*we can leave a tape string which only contains one non-blank unchanged *)
+  Lemma E_rewrite_sym_stay p σ n : valid rewHeadTape (inr (inr (p, Some σ)) :: E p (S (S n))) (inr (inr (∘ (Some σ))) :: E neutral (S (S n))).  
+  Proof. 
+    constructor 3. 
+    - apply E_rewrite_blank. 
+    - cbn[E]. apply rewritesHeadInd_rem_tail. eauto. 
+  Qed. 
+
+  (*we can add a symbol at the head of an empty tape string *)
+  Lemma E_rewrite_sym p σ n: valid rewHeadTape (E p (S (S (S n)))) (inr (inr (positive, Some σ)) :: E positive (S (S n))). 
+  Proof. 
+    cbn [E].
+    constructor 3. 
+    - apply E_rewrite_blank. 
+    - eauto. 
+  Qed. 
+
+  Lemma E_rewrite_sym_unique p σ n : forall (s : string Gamma), valid rewHeadTape (E p (S (S (S n)))) (inr (inr (positive, σ)) :: s) -> s = E positive (S (S n)). 
+  Proof. 
+    intros. inv_valid. rewHeadTape_inv2.
+    all: cbn [E]; f_equal; apply E_rewrite_blank_unique in H3; auto. 
+  Qed. 
+
+  Lemma E_rewrite_sym_rev p σ n : valid rewHeadTape (rev (E p (S (S (S n))))) (rev (inr (inr (negative, Some σ)) :: E negative (S (S n)))). 
+  Proof. 
+    (*follows using tape_rewrite_symm1, tape_rewrite_symm3 and E_rewrite_sym *)
+    specialize (E_rewrite_sym p σ n) as H1. 
+    eapply tape_rewrite_symm1 in H1. 
+    eapply tape_rewrite_symm3 in H1.
+    unfold polarityRev in H1. rewrite map_rev, map_map in H1. setoid_rewrite polarityFlipGamma_involution in H1. rewrite map_id in H1. 
+    cbn [map polarityFlipGamma polarityFlipTapeSigma polarityFlipSigma polarityFlip] in H1. 
+    now rewrite E_polarityFlip in H1. 
+  Qed. 
+
+  Lemma E_rewrite_sym_rev_unique p σ n : forall s, valid rewHeadTape (rev (E p (S (S (S n))))) (rev (inr (inr (negative, Some σ)) :: s)) -> s = E negative (S (S n)). 
+  Proof. 
+    intros.
+    assert (valid rewHeadTape (polarityRev (E (polarityFlip p) (S (S (S n))))) (polarityRev (inr (inr (positive, Some σ)) :: map polarityFlipGamma s))). 
+    {
+      unfold polarityRev. rewrite E_polarityFlip. cbn. rewrite map_involution. 2: involution_simpl.
+      specialize (polarityFlip_involution p) as H1. rewrite H1. apply H. 
+    }
+    eapply tape_rewrite_symm2 in H0.
+    apply E_rewrite_sym_unique in H0. 
+    enough (map polarityFlipGamma (E negative (S (S n))) = E positive (S (S n))).
+    { rewrite <- H1 in H0. apply involution_invert_eqn in H0. assumption. apply map_involution, polarityFlipGamma_involution. }
+    apply E_polarityFlip. 
+  Qed. 
+
+  (*we can also remove a symbol *)
+  Lemma E_rewrite_sym_rem p σ n : valid rewHeadTape (inr (inr (p, Some σ)) :: E p (S (S n))) (E negative (S (S (S n)))). 
+  Proof. 
+    cbn. constructor 3.  
+    - apply E_rewrite_blank.
+    - eauto. 
+  Qed. 
+
+  Lemma  E_rewrite_sym_rem_unique p p' σ n : forall s, valid rewHeadTape (inr (inr (p, Some σ)) :: E p (S (S n))) (inr (inr (p', |_|)):: s) -> p' = negative /\ s = E negative (S (S n)). 
+  Proof. 
+    intros. inv_valid. rewHeadTape_inv2.
+    destruct p'; cbn in H5; try congruence; clear H5.
+    split; [reflexivity | ]. 
+    inv_valid. 1: destruct n; cbn in H5; lia.
+    rewHeadTape_inv2.
+    3: {
+      destruct n; cbn in *; inv H3.
+      apply valid_length_inv in H2; destruct s0; cbn in H2; congruence.
+    }
+    all: destruct n; cbn in H3; [congruence | ];
+      apply E_rewrite_blank_unique in H2;
+      rewrite H2; easy.   
+  Qed. 
+
+  Lemma E_rewrite_sym_rem_rev p σ n : valid rewHeadTape (rev (inr (inr (p, Some σ)) :: E p (S (S n)))) (rev (E positive (S (S (S n))))). 
+  Proof. 
+    specialize (E_rewrite_sym_rem p σ n) as H1. 
+    eapply tape_rewrite_symm1 in H1. 
+    eapply tape_rewrite_symm3 in H1.
+    unfold polarityRev in H1. rewrite map_rev, map_map in H1. setoid_rewrite polarityFlipGamma_involution in H1. rewrite map_id in H1. 
+    cbn [map polarityFlipGamma polarityFlipTapeSigma polarityFlipSigma polarityFlip] in H1. 
+    now rewrite E_polarityFlip in H1. 
+  Qed. 
+
+  Lemma E_rewrite_sym_rem_rev_unique p p' σ n : forall s, valid rewHeadTape (rev (inr (inr (p, Some σ)) :: E p (S (S n)))) (rev (inr (inr (p', |_|)) :: s)) -> p' = positive /\ s = E p' (S (S n)). 
+  Proof. 
+    intros.
+    assert (valid rewHeadTape (polarityRev (inr (inr (polarityFlip p, Some σ)) :: E (polarityFlip p) (S (S n)))) (polarityRev (inr (inr (polarityFlip p', |_|)) :: map polarityFlipGamma s))). 
+    {
+      unfold polarityRev. cbn [map]. rewrite E_polarityFlip. cbn. rewrite map_involution. 2: apply polarityFlipGamma_involution.
+      specialize (polarityFlip_involution) as H1. unfold involution in H1. 
+      rewrite !H1. apply H. 
+    }
+    eapply tape_rewrite_symm2 in H0.
+    apply E_rewrite_sym_rem_unique in H0 as (H0 & H1). 
+    destruct p'; cbn in H0; try congruence; clear H0. 
+    split; [reflexivity | ]. 
+    enough (map polarityFlipGamma (E negative (S (S n))) = E positive (S (S n))).
+    { rewrite <- H1 in H0. rewrite map_involution in H0; [apply H0 | involution_simpl]. }
+    apply E_polarityFlip. 
+  Qed. 
+
+  (** *the following results generalise Lemma 15 *)
+
+  (*Lemma 18 *)
+  (*we can add a symbol to an arbitrary tape string if there is enough space left *)
+  Lemma tape_repr_add_right rs σ h p w:
+    rs ≃t(p, w) h -> length rs < w
+    -> exists h', valid rewHeadTape h (inr (inr (↑ (Some σ))) :: h')
+            /\ (forall h0, valid rewHeadTape h (inr (inr (↑ (Some σ))) :: h0) -> h0 = h')
+            /\ σ :: rs ≃t(positive, w)  (inr (inr (↑ (Some σ))) :: h').
+  Proof. 
+    intros. revert w h σ H H0. 
+    induction rs.
+    - intros. destruct_tape_in_tidy H.
+      exists (E positive (wo + w - 1)). rewrite <- and_assoc; split.
+      + cbn in H0. destruct w; [lia | ]. unfold wo.
+        replace (2 + S w) with (S (S (S w))) by lia. cbn [Nat.sub]. split.
+        * (*existence*) apply E_rewrite_sym.
+        * (*uniqueness*) intros. eapply E_rewrite_sym_unique with (σ := Some σ), H1. 
+      + repeat split. 
+        * cbn. rewrite E_length. lia. 
+        * now cbn. 
+    - intros. apply tape_repr_inv6 in H as (h' & n & -> & -> & H2 & H3).
+      replace (n + S (|h'|) - 1) with (n + |h'|) in H3 by lia.
+      destruct rs; [ | destruct rs].
+      + (*at the end of the used tape region *)
+        destruct h'; [clear H2 | now cbn in H2]. clear H3.
+        destruct n; [cbn in H0; cbn in H0; lia | ].
+        exists (inr (inr ((↑ (Some a)))):: E positive (wo + n)). rewrite <- and_assoc; split.
+        * cbn. split.
+          ++ (*existence*) constructor 3. 
+             -- apply E_rewrite_sym. 
+             -- apply rewritesHeadInd_rem_tail. eauto. 
+          ++ (*uniqueness *) intros. inv_valid.
+             rewHeadTape_inv2. apply E_rewrite_sym_unique with (σ := Some a) in H4. now inv H4. 
+        * repeat split; cbn. 
+          -- rewrite E_length. cbn in H0. lia. 
+          -- cbn in H0; lia. 
+          -- now rewrite Nat.add_comm.
+      + (* rs has length 1*)
+        destruct_tape. cbn [app] in H3. 
+        destruct h'; [ | now cbn in H2]. clear H2.
+        cbn [app] in H3. destruct_tape. cbn [length] in *.
+        destruct n; [lia | ]. clear H0. 
+        exists (inr(inr (↑ (Some a))) :: inr (inr (↑ (Some e))) :: E positive (wo + n)). 
+        cbn [app]; rewrite <- and_assoc; split. 
+        * split.
+          ** (*existence*) constructor 3. 
+              -- replace (2 + S n) with (S(S (S n))) by lia. constructor 3. 
+                ++ apply E_rewrite_sym. 
+                ++ cbn [E]. apply rewritesHeadInd_rem_tail; eauto. 
+              -- cbn[E]. apply rewritesHeadInd_rem_tail. eauto. 
+          ** (*uniqueness*)
+            intros. inv_valid. rewHeadTape_inv2. 
+            inv_valid. rewHeadTape_inv2. 
+            apply E_rewrite_sym_unique in H2. 
+            cbn [E] in H2. inv H2. inv H3. reflexivity.  
+        * repeat split.
+          -- cbn. rewrite E_length. lia. 
+          -- cbn; lia. 
+          -- cbn[mapPolarity map length app]. now replace (wo + (S n + 2) - 3) with (wo + n) by lia. 
+     + (*rs has at least two elements. this is the interesting case as it needs the IH *) 
+       destruct_tape. cbn [app] in H3. cbn [length app] in H3. rewrite Nat.add_succ_r in H3. 
+       apply tape_repr_step in H3 as H4. destruct_tape. cbn [app length] in *. destruct_tape. 
+
+       (*we use the IH with h := inr (...e) :: inr (...e0) :: h' ++ E(n + wo); w := S (S (n + |h'|)); σ := a *)
+       rewrite Nat.add_succ_r in H3. specialize (IHrs _ _ a H3). 
+       edestruct (IHrs) as (h'' & F1 & F3 & F2). lia. 
+       exists (inr (inr (↑(Some a))) :: h'').
+       (*we need to know one more symbol at the head of h'' for the proof *)
+       destruct_tape_in F2. 
+       rewrite <- and_assoc; split; [split | ].
+       * (*existence*)constructor 3.  
+         -- apply F1. 
+         -- apply rewritesHeadInd_rem_tail; eauto. 
+       * (*uniqueness*)
+         intros. clear IHrs. inv_valid. rewHeadTape_inv2. apply F3 in H7. inv H7. reflexivity. 
+       * repeat split.
+         -- cbn; destruct F2 as (F2 & _ & _). cbn in F2. lia.  
+         -- cbn; destruct F2 as (_ & F2 & _). cbn in F2. lia. 
+         -- destruct F2 as (_ & _ & ->). cbn[app length Nat.add Nat.sub].
+            replace (wo + (n + S (S (S (|h'|)))) - (S (S (S (S(|rs|)))))) with (wo + S (S (n + (|h'|))) - S (S (S(|rs|)))) by lia.
+            easy. 
+  Qed. 
+
+  (*the same result for the left tape half can be derived using the symm lemmas*)
+  Corollary tape_repr_add_left ls σ h p w:
+    ls ≃t(p, w) h -> length ls < w
+    -> exists h', valid rewHeadTape (rev h) (rev (inr (inr (↓ (Some σ))) :: h'))
+            /\ (forall h0, valid rewHeadTape (rev h) (rev (inr (inr (↓ (Some σ))) :: h0)) -> h0 = h')
+            /\ σ :: ls ≃t(negative, w)  (inr (inr (↓ (Some σ))) :: h').
+  Proof. 
+    intros. specialize (@tape_repr_add_right ls σ h p w H H0) as (h' & H1 & H3 & H2). 
+    exists (map polarityFlipGamma h'). rewrite <- and_assoc. split. 
+    - eapply tape_rewrite_symm1 in H1.  
+      apply tape_rewrite_symm3 in H1. split. 
+      + cbn in *. unfold polarityRev in H1. rewrite map_rev in H1. rewrite map_involution in H1.
+        2: apply polarityFlipGamma_involution.
+        apply H1. 
+      + intros. specialize (H3 (map polarityFlipGamma h0)).
+        rewrite <- involution_invert_eqn2 with (f := map polarityFlipGamma) (a := h0) (b := h'); [reflexivity | apply map_involution, polarityFlipGamma_involution | ]. 
+        apply H3. eapply tape_rewrite_symm2. 
+        unfold polarityRev. rewrite <- map_rev. apply tape_rewrite_symm3. 
+        cbn. rewrite map_involution; [now apply H4 | apply polarityFlipGamma_involution]. 
+   - apply tape_repr_polarityFlip in H2. cbn in H2. easy. 
+  Qed. 
+
+  (*Lemma 19*)
+  (*we can remove a symbol from the right tape half *)
+  (*this is a weaker version where we know that the second symbol (the new head symbol) is not a blank *)
+  (*the general version will be derived from this *)
+  Lemma tape_repr_rem_right' rs σ1 σ2 (h : list Gamma) p w :
+    σ1 :: σ2 :: rs ≃t(p, w) inr (inr (p, Some σ1)) :: inr (inr (p, Some σ2)) :: h
+    -> exists (h' : list Gamma), valid rewHeadTape (inr (inr (p, Some σ1)) :: inr (inr (p, Some σ2)) :: h) (inr (inr (↓ (Some σ2))) :: h')
+                           /\ (forall h0, valid rewHeadTape (inr (inr (p, Some σ1)) :: inr (inr (p, Some σ2)) :: h) (inr (inr (↓ (Some σ2))) :: h0) -> h0 = h')
+                           /\ σ2 :: rs ≃t(negative, w) (inr (inr (↓ (Some σ2))) :: h').
+  Proof. 
+    revert w h σ1 σ2. 
+    induction rs. 
+    - intros. destruct_tape. exists (E negative (S wo + w)). rewrite <- and_assoc; split. 
+      + (* existence*) split.
+        * constructor 3.
+          -- constructor 3.
+             ++ apply E_rewrite_blank. 
+             ++ apply rewritesHeadInd_rem_tail. eauto. 
+          -- apply rewritesHeadInd_rem_tail. eauto. 
+        * (*uniqueness *) intros. do 2 (inv_valid; rewHeadTape_inv2).  
+           apply E_rewrite_blank_unique in H3. inv H3. now cbn. 
+      + (*correctness*)
+        repeat split.
+        * cbn. rewrite E_length. lia. 
+        * now cbn.
+  - intros. destruct_tape_in H. 
+    destruct rs. 
+    + destruct_tape_in H. 
+      exists (inr (inr (↓ (Some a))) :: E negative (S wo + w)). rewrite <- and_assoc; split. 
+      * split. 
+        -- constructor 3.
+           ++ constructor 3. { apply E_rewrite_sym_rem. }
+              apply rewritesHeadInd_rem_tail. eauto.  
+           ++ apply rewritesHeadInd_rem_tail. eauto.
+        -- (* uniqueness*) intros.  
+           inv_valid. rewHeadTape_inv2; [inv_valid; rewHeadTape_inv2 | ].
+           do 2 inv_valid; rewHeadTape_inv2. 
+           apply E_rewrite_blank_unique in H4. inv H4. cbn [E]; easy. 
+      * (*correctness *)
+        repeat split. 
+        -- cbn [length]. rewrite E_length. lia. 
+        -- now cbn.
+    + destruct_tape.
+      (*need IH *)
+      apply tape_repr_step in H. 
+      specialize (IHrs _ _ σ2 a H) as (h0 & F1 & F2 & F3). destruct_tape. 
+      exists (inr (inr (↓ (Some a))) :: (inr (inr (↓ (Some e)))) :: h0). 
+      rewrite <- and_assoc; split; [split | ]. 
+      * constructor 3.
+        -- apply F1. 
+        -- apply rewritesHeadInd_rem_tail. eauto. 
+      * (*uniqueness *)intros. inv_valid. rewHeadTape_inv2; apply F2 in H4; now inv H4. 
+      * clear F2 F1 H. destruct F3 as (H1 & H2 & H3). repeat split.
+        -- cbn in *. lia. 
+        -- cbn in *; lia. 
+        -- inv H3. easy. 
+  Qed.      
+
+  Lemma tape_repr_rem_right rs σ (m : stateSigma) h p w :
+    σ :: rs ≃t(p, w) inr (inr (p, Some σ)) :: inr (inr (p, m)) :: h
+    -> exists h', valid rewHeadTape (inr (inr (p, Some σ)) :: inr (inr (p, m)) :: h) (inr (inr (negative, m)) :: h')
+            /\ (forall h0, valid rewHeadTape (inr (inr (p, Some σ)) :: inr (inr (p, m)) :: h) (inr (inr (negative, m)) :: h0) -> h0 = h' )
+            /\ rs ≃t(negative, w) (inr (inr (negative, m)) :: h').
+  Proof. 
+    intros. destruct m as [σ2 | ].
+    + inv_tape' H.
+      now apply tape_repr_rem_right'.
+    + destruct_tape_in_tidy H.
+      apply tape_repr_step in H as H'. destruct_tape_in_tidy H'. clear H'.
+      exists (E negative (wo + w)). repeat split. 
+      * constructor 3; [apply E_rewrite_blank | cbn; eauto ].
+      * intros. inv_valid. rewHeadTape_inv2. 
+        apply E_rewrite_blank_unique in H4. now inv H4.  
+      * cbn; now rewrite E_length. 
+      * now cbn. 
+  Qed.
+
+  Corollary tape_repr_rem_left ls σ (m : stateSigma) h p w :
+    σ :: ls ≃t(p, w) inr (inr (p, Some σ)) :: inr (inr (p, m)) :: h
+    -> exists h', valid rewHeadTape (rev (inr (inr (p, Some σ)) :: inr (inr (p, m)) :: h)) (rev (inr (inr (positive, m)) :: h'))
+            /\ (forall h0, valid rewHeadTape (rev (inr (inr (p, Some σ)) :: inr (inr (p, m)) :: h)) (rev (inr (inr (positive, m)) :: h0)) -> h0 = h')
+            /\ ls ≃t(positive, w) (inr (inr (positive, m)) :: h').
+  Proof. 
+    intros. specialize (@tape_repr_rem_right ls σ m h p w H) as (h' & H1 & H3 & H2). 
+    exists (map polarityFlipGamma h'). rewrite <- and_assoc. split. 
+    - eapply tape_rewrite_symm1 in H1. apply tape_rewrite_symm3 in H1.
+      split. 
+      + unfold polarityRev in H1. rewrite map_rev in H1. rewrite map_involution in H1. 2: apply polarityFlipGamma_involution.  destruct m; cbn in H1; cbn; apply H1.
+      + intros. specialize (H3 (map polarityFlipGamma h0)).
+        rewrite <- involution_invert_eqn2 with (f := map polarityFlipGamma) (a := h0) (b := h'); [reflexivity | apply map_involution, polarityFlipGamma_involution | ]. 
+        apply H3. eapply tape_rewrite_symm2. 
+        unfold polarityRev. rewrite <- map_rev. apply tape_rewrite_symm3. 
+        cbn in *. rewrite map_involution; [destruct m; cbn in *; now apply H0 | apply polarityFlipGamma_involution]. 
+   - apply tape_repr_polarityFlip in H2. destruct m; cbn in H2; easy. 
+  Qed. 
+
+
+  (*Lemma 20*)
+  (*we can leave tape strings unchanged (mod polarity) *)
+  Lemma tape_repr_stay_right' rs σ h p w :
+    σ :: rs ≃t(p, w) inr(inr (p, Some σ)) :: h
+    -> exists h', valid rewHeadTape (inr (inr (p, Some σ)) :: h) (inr (inr (neutral, Some σ)) :: h')
+            /\ (forall h0, valid rewHeadTape (inr (inr (p, Some σ)) :: h) (inr (inr (∘ (Some σ))) :: h0) -> h0 = h')
+            /\ σ :: rs ≃t(neutral, w) (inr (inr (∘ (Some σ)))) :: h'.
+  Proof. 
+    revert w h σ.  
+    induction rs. 
+    - intros. destruct_tape. exists (E neutral (wo + w)). 
+      rewrite <- and_assoc. split. 
+      + split.
+        * constructor 3. apply E_rewrite_blank.
+          apply rewritesHeadInd_rem_tail. eauto. 
+        * intros. inv_valid.  
+          rewHeadTape_inv2. apply E_rewrite_blank_unique in H4. inv H4. easy. 
+      + repeat split; cbn in *; try rewrite E_length; cbn in *; easy. 
+    - intros. destruct_tape_in H. destruct rs; destruct_tape_in H. 
+      + exists (inr (inr (∘ (Some a))) :: E neutral (wo + w)). rewrite <- and_assoc; split. 
+        * split.
+          -- constructor 3. 2: { apply rewritesHeadInd_rem_tail. eauto. }
+             apply E_rewrite_sym_stay. 
+          -- intros. do 2 (inv_valid; rewHeadTape_inv2). 
+             apply E_rewrite_blank_unique in H3. inv H3. easy. 
+        * repeat split; cbn in *; try rewrite E_length; cbn in *; easy.  
+     + apply tape_repr_step in H. specialize (IHrs _ _ a H) as (h0 & F1 & F2 & F3). destruct_tape_in F3. 
+       exists (inr (inr (∘ (Some a))) :: inr (inr (∘ (Some e))) :: h0). rewrite <- and_assoc; split.
+       * split.
+         -- constructor 3.
+            ++ apply F1. 
+            ++ apply rewritesHeadInd_rem_tail; eauto. 
+         -- intros. inv_valid. rewHeadTape_inv2. apply F2 in H4. inv H4. easy. 
+       * clear F2 F1 H. destruct F3 as (H1 & H2 & H3). cbn in H1, H2. repeat split; cbn. 1-2: lia. inv H3. easy. 
+  Qed. 
+
+  Lemma tape_repr_stay_right rs e h p w :
+    rs ≃t(p, w) inr (inr (p, e)) :: h
+    -> exists h', valid rewHeadTape (inr (inr (p, e)) :: h) (inr (inr (neutral, e)) :: h')
+            /\ (forall h0, valid rewHeadTape (inr (inr (p, e)) :: h) (inr (inr (neutral, e)) :: h0) -> h0 = h')
+            /\ rs ≃t(neutral, w) (inr (inr (neutral, e)) :: h').
+  Proof.
+    intros. destruct e. 
+    - cbn in H. destruct_tape_in H. now apply tape_repr_stay_right'. 
+    - cbn in H. destruct_tape_in_tidy H. exists (inr (inr (neutral, |_|)) :: E neutral w). split; [ | split]. 
+      + apply E_rewrite_blank.
+      + intros. apply E_rewrite_blank_unique in H0. now inv H0. 
+      + repeat split; cbn; [rewrite E_length | ]; lia.
+  Qed. 
+
+  Corollary tape_repr_stay_left ls e h p w :
+    ls ≃t(p, w) inr(inr (p, e)) :: h
+    -> exists h', valid rewHeadTape (rev (inr (inr (p, e)) :: h)) (rev (inr (inr (neutral, e)) :: h'))
+            /\ (forall h0, valid rewHeadTape (rev (inr (inr (p, e)) :: h)) (rev (inr (inr (neutral, e)) :: h0)) -> h0 = h')
+            /\ ls ≃t(neutral, w) (inr (inr (neutral, e))) :: h'.
+  Proof. 
+    intros. specialize (@tape_repr_stay_right ls e h p w H) as (h' & H1 & H3 & H2). 
+    exists (map polarityFlipGamma h'). rewrite <- and_assoc. split. 
+    - eapply tape_rewrite_symm1 in H1.
+      apply tape_rewrite_symm3 in H1.
+      split. 
+      + cbn [rev].
+        unfold polarityRev in H1. rewrite map_rev in H1. rewrite map_involution in H1. 2: apply polarityFlipGamma_involution. 
+        destruct e; cbn in H1; apply H1. 
+      + intros. specialize (H3 (map polarityFlipGamma h0)).
+        rewrite <- involution_invert_eqn2 with (f := map polarityFlipGamma) (a := h0) (b := h'); [reflexivity | apply map_involution, polarityFlipGamma_involution | ]. 
+        apply H3. eapply tape_rewrite_symm2. 
+        unfold polarityRev. rewrite <- map_rev. apply tape_rewrite_symm3. 
+        cbn. rewrite map_involution; [destruct e; cbn; now apply H0 | apply polarityFlipGamma_involution]. 
+   - apply tape_repr_polarityFlip in H2. destruct e; cbn in H2; easy. 
+  Qed. 
+
+End tape.
